rename algorithms with more consistent naming schemes.

OL_Reflection_2_memo.v
@@ -3,6 +3,7 @@ Require Import OL_Theory.
 
 Require Import OL_Reflection_1_base.
 
+
 Require Import Setoid Morphisms.
 Require Import Lia.
 Require Import Coq.Arith.Bool_nat.
@@ -47,7 +48,7 @@ Fixpoint find (x: MemoKey) (l: MemoMap) : option (MemoKey * bool) := match l wit
 | head :: tail => if MemoKey_eqdec x (fst head) then Some head else find x tail
 end.
 
-Fixpoint decideOL_boolM (fuel: nat) (g d: AnTerm) (memo: MemoMap) : (bool * MemoMap) :=
+Fixpoint decideOL_memo (fuel: nat) (g d: AnTerm) (memo: MemoMap) : (bool * MemoMap) :=
 match find (g, d) memo with
 | Some (_, b) => (b, memo)
 | None => (match fuel with
@@ -56,68 +57,64 @@ match find (g, d) memo with
     (* Guaranteed sufficent cases. *)
       match (g, d) with 
       | (L (Var a), R (Var b) )  => Mbool (Pos.eqb a b) (* Hyp *)
-      (*| (L (Meet a b), N) => decideOL_boolM n (L a) (L b) (* LeftAnd1-2 *)*)
-      (*| (N, R (Join a b)) => decideOL_boolM n (R a) (R b) (* RightOr1-2 *)*)
-      | (L (Join a b), _) => (decideOL_boolM n (L a) d) &&& (decideOL_boolM n (L b) d) (* LeftOr *)
-      | (L (Not a), _) => decideOL_boolM n (R a) d (* LeftNot *)
-      | (_, R (Meet a b)) => (decideOL_boolM n g (R a)) &&& (decideOL_boolM n g (R b)) (* RightAnd *)
-      | (_, R (Not a)) => decideOL_boolM n g (L a) (* RightNot *)
+      | (L (Join a b), _) => (decideOL_memo n (L a) d) &&& (decideOL_memo n (L b) d) (* LeftOr *)
+      | (L (Not a), _) => decideOL_memo n (R a) d (* LeftNot *)
+      | (_, R (Meet a b)) => (decideOL_memo n g (R a)) &&& (decideOL_memo n g (R b)) (* RightAnd *)
+      | (_, R (Not a)) => decideOL_memo n g (L a) (* RightNot *)
           (* Swap cases *)
       | (R (Var a), L (Var b) )  => Mbool (Pos.eqb b a) (* Hyp *)
-      (*| (N, L (Meet a b)) => decideOL_boolM n (L a) (L b) (* LeftAnd1-2 *)*)
-      (*| (R (Join a b), N) => decideOL_boolM n (R a) (R b) (* RightOr1-2 *)*)
-      | (_, L (Join a b)) => (decideOL_boolM n g (L a)) &&& (decideOL_boolM n g (L b)) (* LeftOr *)
-      | (_, L (Not a)) => decideOL_boolM n g (R a) (* LeftNot *)
-      | (R (Meet a b), _) => (decideOL_boolM n (R a) d) &&& (decideOL_boolM n (R b) d) (* RightAnd *)
-      | (R (Not a), _) => decideOL_boolM n (L a) d (* RightNot *)
+      | (_, L (Join a b)) => (decideOL_memo n g (L a)) &&& (decideOL_memo n g (L b)) (* LeftOr *)
+      | (_, L (Not a)) => decideOL_memo n g (R a) (* LeftNot *)
+      | (R (Meet a b), _) => (decideOL_memo n (R a) d) &&& (decideOL_memo n (R b) d) (* RightAnd *)
+      | (R (Not a), _) => decideOL_memo n (L a) d (* RightNot *)
       | _ => 
                 match d with (* Weaken g*)
-        | L a => decideOL_boolM n g N 
-        | R a => decideOL_boolM n g N 
+        | L a => decideOL_memo n g N 
+        | R a => decideOL_memo n g N 
         | N => Mfalse
         end |||(
         match g with (* Weaken d*)
-        | L a => decideOL_boolM n d N 
-        | R a => decideOL_boolM n d N 
+        | L a => decideOL_memo n d N 
+        | R a => decideOL_memo n d N 
         | N => Mfalse
         end |||(
         match g with (* LeftAnd1 g*)
-        | L (Meet a b) => decideOL_boolM n (L a) d
+        | L (Meet a b) => decideOL_memo n (L a) d
         | _ => Mfalse
         end |||(
         match d with (* LeftAnd1 d*)
-        | L (Meet a b) => decideOL_boolM n (L a) g
+        | L (Meet a b) => decideOL_memo n (L a) g
         | _ => Mfalse
         end |||(
         match g with (* LeftAnd2 g*)
-        | L (Meet a b) => decideOL_boolM n (L b) d
+        | L (Meet a b) => decideOL_memo n (L b) d
         | _ => Mfalse
         end |||(
         match d with (* LeftAnd2 d*)
-        | L (Meet a b) => decideOL_boolM n (L b) g
+        | L (Meet a b) => decideOL_memo n (L b) g
         | _ => Mfalse
         end |||(
         match g with (* RightOr1 g*)
-        | R (Join a b) => decideOL_boolM n d (R a)
+        | R (Join a b) => decideOL_memo n d (R a)
         | _ => Mfalse
         end |||(
         match d with (* RightOr1 d*)
-        | R (Join a b) => decideOL_boolM n g (R a)
+        | R (Join a b) => decideOL_memo n g (R a)
         | _ => Mfalse
         end |||(
         match g with (* RightOr2 g*)
-        | R (Join a b) => decideOL_boolM n d (R b)
+        | R (Join a b) => decideOL_memo n d (R b)
         | _ => Mfalse
         end |||(
         match d with (* RightOr2 d*)
-        | R (Join a b) => decideOL_boolM n g (R b)
+        | R (Join a b) => decideOL_memo n g (R b)
         | _ => Mfalse
         end |||(
         match (g, d) with
-        | (N, L(_)) => decideOL_boolM n d d
-        | (N, R(_)) => decideOL_boolM n d d
-        | (L(_), N) => decideOL_boolM n g g
-        | (R(_), N) => decideOL_boolM n g g
+        | (N, L(_)) => decideOL_memo n d d
+        | (N, R(_)) => decideOL_memo n d d
+        | (L(_), N) => decideOL_memo n g g
+        | (R(_), N) => decideOL_memo n g g
         | _ => Mfalse
         end
         ))))))))))
@@ -126,13 +123,11 @@ match find (g, d) memo with
 end.
 
 
-Definition decideOL_boolMemo (g d: AnTerm): bool := fst (decideOL_boolM (anSize g * anSize d + 4) g d []).
-
-Definition decideOL_bool_simp (g d: AnTerm): bool := decideOL_bool (anSize g + anSize d) g d.
+Definition decideOL_memo_simp (g d: AnTerm): bool := fst (decideOL_memo (anSize g * anSize d + 4) g d []).
 
 Definition correctMemoMap (l: MemoMap) :=  forall g d, 
   match find (g, d) l with
-  | Some (_, true) => exists n,  (decideOL_bool n g d = true)
+  | Some (_, true) => exists n,  (decideOL_base n g d = true)
   | _ => True
   end.
 
@@ -188,7 +183,7 @@ Qed.
 Ltac dest g := destruct g; try congruence.
 
 (*
-Theorem decideOL_bool_big_fuel  : forall n n0 g d, (n >= anSize g + anSize d) -> ( n0 >= anSize g + anSize d) -> decideOL_bool n g d = decideOL_bool n0 g d.
+Theorem decideOL_base_big_fuel  : forall n n0 g d, (n >= anSize g + anSize d) -> ( n0 >= anSize g + anSize d) -> decideOL_base n g d = decideOL_base n0 g d.
 Proof.
   induction n. intros. pose proof anSizePositive g; pose proof anSizePositive d. lia.
   induction n0. intros. pose proof anSizePositive g; pose proof anSizePositive d. lia.
@@ -233,13 +228,13 @@ Qed.
 Lemma correctMemoAdditionEq2 g d l e : 
   (*(n >= anSize g + anSize d) -> *)
   correctMemoMap l -> 
-  (e = true -> exists n, decideOL_bool n g d = true) -> 
+  (e = true -> exists n, decideOL_base n g d = true) -> 
   correctMemoMap ((g, d, e) :: l).
 Proof.
   intros. unfold correctMemoMap. intros.
   unfold find. fold find. destruct e.
-  - destruct H0 as [n H0]; auto.  destruct (MemoKey_eqdec (g0, d0) (fst (g, d, decideOL_bool n g d))).
-    + rewrite MemoKey_eqdec_refl; auto. exists n. destruct (decideOL_bool n g d) eqn: res; simpl in *.
+  - destruct H0 as [n H0]; auto.  destruct (MemoKey_eqdec (g0, d0) (fst (g, d, decideOL_base n g d))).
+    + rewrite MemoKey_eqdec_refl; auto. exists n. destruct (decideOL_base n g d) eqn: res; simpl in *.
       intros. simpl in *.  assert (g0 = g). congruence. assert (d0 = d). congruence. subst. auto. exfalso. auto with *.
     + rewrite MemoKey_eqdec_refl2. 2: auto. apply H.
   - destruct (MemoKey_eqdec (g0, d0) (fst (g, d, false))).
@@ -270,7 +265,7 @@ Proof.
 Qed.
 
 (*
-Theorem decideOL_bool_big_fuel  : forall n n0 g d, (n >= anSize g + anSize d) -> ( n0 >= anSize g + anSize d) -> decideOL_bool n g d = decideOL_bool n0 g d.
+Theorem decideOL_base_big_fuel  : forall n n0 g d, (n >= anSize g + anSize d) -> ( n0 >= anSize g + anSize d) -> decideOL_base n g d = decideOL_base n0 g d.
 Proof.
   induction n. intros. pose proof anSizePositive g; pose proof anSizePositive d. lia.
   induction n0. intros. pose proof anSizePositive g; pose proof anSizePositive d. lia.
@@ -299,27 +294,11 @@ Proof.
 Qed.
 
 
-
-Lemma decideOL_bool_monotonic : forall (n2 n1: nat) g d, n2 >= n1 -> decideOL_bool n1 g d = true -> decideOL_bool n2 g d = true.
-Proof.
-  induction n2.
-  - intros. simpl in *. assert (n1 = 0). lia. subst. simpl in *. congruence.
-  - intros. destruct n1. simpl in *; congruence. destruct g as [ | t | t ]; try destruct t.
-    all: try destruct d as [ | t0 | t0 ]; try destruct t0; simpl; simpl in H0.
-      all: repeat rewrite Bool.orb_false_r in *; repeat rewrite Bool.orb_true_iff in *; repeat rewrite Bool.andb_true_iff in *; auto.
-      all: repeat match goal with
-      | [H: _ \/ _ |- _] => destruct H; only 1: left; only 2: right
-      | [H: _ /\ _ |- _] => destruct H; split
-      | _ => idtac
-      end. all: apply (IHn2 n1); try lia; auto.
-Qed.
-
-
-Theorem decideOLBoolMemoCorrect : 
+Theorem decideOL_memo_Correct : 
   forall n g d l, 
   (correctMemoMap l) -> 
-  (correctMemoMap (snd (decideOL_boolM n g d l))) /\
-  (((fst (decideOL_boolM n g d l)) = true) ->  exists n0, (decideOL_bool n0 g d) = true).
+  (correctMemoMap (snd (decideOL_memo n g d l))) /\
+  (((fst (decideOL_memo n g d l)) = true) ->  exists n0, (decideOL_base n0 g d) = true).
 Proof.
   induction n.
   - intros. split.
@@ -345,10 +324,10 @@ Proof.
         assert ((x &&& y) l = let (b, m) := x l in if b then (y m) else (false, m) ) as rew_first_and; (only 1: reflexivity); rewrite rew_first_and in *; clear rew_first_and.
 
       (* recursively prove goals of the form 
-            correctMemoMap (snd (decideOL_boolM n g1 d1 ||| (decideOL_boolM n g2 d2||| (decideOL_boolM n g3 d3 ||| ... ))) )
+            correctMemoMap (snd (decideOL_memo n g1 d1 ||| (decideOL_memo n g2 d2||| (decideOL_memo n g3 d3 ||| ... ))) )
         and
-            fst ( (decideOL_boolM n g1 d1 ||| (decideOL_boolM n g2 d2||| (decideOL_boolM n g3 d3 ||| ... ))) l) =
-                        (decideOL_bool n g1 d1 ||| (decideOL_bool n g2 d2||| (decideOL_bool n g3 d3 ||| ... )))
+            fst ( (decideOL_memo n g1 d1 ||| (decideOL_memo n g2 d2||| (decideOL_memo n g3 d3 ||| ... ))) l) =
+                        (decideOL_base n g1 d1 ||| (decideOL_base n g2 d2||| (decideOL_base n g3 d3 ||| ... )))
         as well as conjunctions
       *)
       Ltac reduceAndOr rest IHn l H :=
@@ -356,28 +335,28 @@ Proof.
         let IHn_fst := (fresh "IHn_fst") in let n0 := (fresh "n0") in 
         let b_ := (fresh "b") in let l_ := (fresh "l") in let found := (fresh "found") in
           lazymatch rest with 
-          | (decideOL_boolM ?n ?g ?d) ||| ?rest2 => 
-            try rewriteOr (decideOL_boolM n g d) rest2 l;
+          | (decideOL_memo ?n ?g ?d) ||| ?rest2 => 
+            try rewriteOr (decideOL_memo n g d) rest2 l;
             pose proof (IHn g d l H) as IHn_; simpl in *; destruct IHn_ as [IHn_snd IHn_fst];
-            destruct (decideOL_boolM n g d l)  as [ b_ l_] eqn: found;
+            destruct (decideOL_memo n g d l)  as [ b_ l_] eqn: found;
             destruct b_; simpl in *; auto;
             intros;
-            try(destruct IHn_fst as [n0 IHn_fst]; auto; exists (S n0); eauto);
+            try(destruct IHn_fst as [n0 IHn_fst]; auto; exists (S n0); eauto using 1);
             simpl in *;
             repeat rewrite Bool.orb_false_r;  repeat rewrite OrMemo_Mfalse_r; repeat rewrite OrMemo_Mfalse_l; repeat rewrite AndMemo_Mfalse_l;
             match goal with | [ |- (_ -> _) ] => intro  | _ => idtac end;
             try congruence;
             try (apply Bool.orb_true_iff; left; congruence);
             try (apply Bool.orb_true_iff; right);
-            try (eapply IHn; simpl in *; eauto; fail); 
-            try (eapply IHn_fst; simpl in *; eauto; fail);
+            try (eapply IHn; simpl in *; eauto using 1; fail); 
+            try (eapply IHn_fst; simpl in *; eauto using 1; fail);
             try (rewrite IHn_fst; simpl; repeat rewrite Bool.orb_true_r; auto;  fail);
             reduceAndOr rest2 IHn l_ IHn_snd;
             idtac
-          | (decideOL_boolM ?n ?g ?d) &&& ?rest2 => 
-            try rewriteAnd (decideOL_boolM n g d) rest2 l;
+          | (decideOL_memo ?n ?g ?d) &&& ?rest2 => 
+            try rewriteAnd (decideOL_memo n g d) rest2 l;
             pose proof (IHn g d l H) as IHn_; simpl in *; destruct IHn_ as [IHn_snd IHn_fst];
-            destruct (decideOL_boolM n g d l)  as [ b_ l_] eqn: found;
+            destruct (decideOL_memo n g d l)  as [ b_ l_] eqn: found;
             destruct b_; simpl in *; auto;
             intros; try congruence;
             match goal with
@@ -388,27 +367,27 @@ Proof.
             simpl in *;
             repeat rewrite Bool.orb_false_r;  repeat rewrite OrMemo_Mfalse_r; repeat rewrite OrMemo_Mfalse_l; repeat rewrite AndMemo_Mfalse_l;
             try (apply Bool.andb_true_iff; split);
-            try (eapply IHn; simpl in *; eauto; fail); 
-            try (eapply IHn_fst; simpl in *; eauto; fail);
+            try (eapply IHn; simpl in *; eauto using 1; fail); 
+            try (eapply IHn_fst; simpl in *; eauto using 1; fail);
             try (rewrite IHn_fst; simpl; repeat rewrite Bool.orb_true_r; auto;  fail);
             reduceAndOr rest2 IHn l_ IHn_snd;
             idtac
-          | decideOL_boolM ?n ?g ?d =>  
+          | decideOL_memo ?n ?g ?d =>  
             simpl in *; repeat rewrite Bool.orb_false_r; simpl in *; auto; intros; try congruence;
-            try (apply IHn; simpl in *; eauto; congruence);
+            try (apply IHn; simpl in *; eauto using 1; congruence);
             pose proof (IHn g d l H) as IHn_; simpl in *; destruct IHn_ as [IHn_snd IHn_fst]; 
             destruct IHn_fst as [n0 IHn_fst]; auto;
             lazymatch goal with
-            | [ J1: decideOL_bool ?m1 _ _ = true, J2: decideOL_bool ?m2 _ _ = true |- _ ] => 
+            | [ J1: decideOL_base ?m1 _ _ = true, J2: decideOL_base ?m2 _ _ = true |- _ ] => 
                 exists (S (Nat.max m1 m2)); simpl; apply Bool.andb_true_iff; split; 
-                only 1: (apply (decideOL_bool_monotonic (Nat.max m1 m2) m1); try lia); 
-                only 2: (apply (decideOL_bool_monotonic (Nat.max m1 m2) m2); try lia);
+                only 1: (apply (decideOL_base_monotonic (Nat.max m1 m2) m1); try lia); 
+                only 2: (apply (decideOL_base_monotonic (Nat.max m1 m2) m2); try lia);
                 idtac
-            | [ J1: decideOL_bool ?m1 _ _ = true |- _ ] =>  exists (S m1); simpl
+            | [ J1: decideOL_base ?m1 _ _ = true |- _ ] =>  exists (S m1); simpl
             | _ => idtac
             end;
             repeat rewrite Bool.orb_false_r;
-            repeat (apply Bool.orb_true_iff; right); eauto;
+            repeat (apply Bool.orb_true_iff; right); eauto using 1;
             idtac
           | Mfalse => simpl in *; auto; intros; congruence;
             idtac
@@ -426,13 +405,13 @@ Proof.
         reduceAndOr rest IHn (head :: l) H0;
         idtac
       | _ => fail "unknown shape"
-      end; fail). Unshelve. all: exact 1.
+      end; fail).
 
       (* Need to do the second half of the proof, which could be the same as the first *)
-    + Opaque decideOL_bool. simpl. pose proof H as H0. unfold correctMemoMap in H0.  specialize (H0 g d).
+    + Opaque decideOL_base. simpl. pose proof H as H0. unfold correctMemoMap in H0.  specialize (H0 g d).
       destruct (find (g, d) l) eqn: res; simpl in *. destruct p; simpl in *. 
       * destruct b eqn:b_eq; simpl in *; intro; auto; try congruence.
-      * Transparent decideOL_bool. destSimp g; destSimp d; (try destSimp t0); (try destSimp t).
+      * Transparent decideOL_base. destSimp g; destSimp d; (try destSimp t0); (try destSimp t).
         all: rewrite fst_let_simpl; simpl in *; repeat rewrite Bool.orb_false_r; repeat rewrite OrMemo_Mfalse_r; repeat rewrite OrMemo_Mfalse_l.
         all: try ( apply IHn; auto; simpl in *; lia).
         all: try (lazymatch goal with
@@ -443,7 +422,8 @@ Proof.
             | [H : correctMemoMap ?l |- ?inner = true -> _ ] => 
               reduceAndOr (Mbool inner) IHn l H
             | _ => fail "unknown shape"
-            end; fail).
+            end; fail). 
+    Unshelve. all: try exact 1.
 Qed.
 
 
@@ -452,17 +432,17 @@ Qed.
 
 
  (* If the algorithms outputs True, then g is semanticaly smaller than d.*)
-Theorem decideOLBoolMemoCorrect2 : forall g d, (decideOL_boolMemo g d) = true -> AnLeq g d.
+Theorem decideOL_memo_simp_correct : forall g d, (decideOL_memo_simp g d) = true -> AnLeq g d.
 Proof. 
-  intros. assert (squash (OLProof (g, d))). (pose proof decideOLBoolMemoCorrect (anSize g * anSize d + 4) g d []). destruct H0. unfold correctMemoMap; simpl in *; auto.
-  specialize (H1 H). destruct H1 as [n0 H1]. apply decideOLBoolCorrect with n0; auto. 
+  intros. assert (squash (OLProof (g, d))). (pose proof decideOL_memo_Correct (anSize g * anSize d + 4) g d []). destruct H0. unfold correctMemoMap; simpl in *; auto.
+  specialize (H1 H). destruct H1 as [n0 H1]. apply decideOL_base_correct with n0; auto. 
   destruct H0. apply (Soundness (g, d)). auto.
 Qed.
 
 
-Theorem reduceToAlgoMemo {OL: Ortholattice} : forall t1 t2 f, (decideOL_boolMemo (L t1) (R t2)) = true -> ((eval t1 f) <= (eval t2 f)).
+Theorem reduceToAlgoMemo {OL: Ortholattice} : forall t1 t2 f, (decideOL_memo_simp (L t1) (R t2)) = true -> ((eval t1 f) <= (eval t2 f)).
 Proof.
-  intros. assert (AnLeq  (L t1) (R t2)). all: auto using decideOLBoolMemoCorrect2.
+  intros. assert (AnLeq  (L t1) (R t2)). all: auto using decideOL_memo_simp_correct.
 Qed.
 
 
